Grandpa/src/Message.v
@@ -1,0 +1,80 @@
+Require Import Blocks.
+Require Import Votes.
+Require Import Dictionary.
+
+Require Import Nat.
+Require Import Coq.Arith.Arith.
+Require Import List.
+
+Variant MessageKind : Type
+  :=
+  | PreCommitMessage : MessageKind
+  | PreViewMessage : MessageKind
+  | EstimateMessage: MessageKind
+  | FinalizationMessage: MessageKind.
+
+Record Message :=
+   { id:nat 
+    ;block:{n & Block n}
+    ;kind: MessageKind
+    ;round:nat
+    ;time:nat
+    ;voter:Voter
+    ;processed_by:Dictionary Voter Unit
+   }.
+
+Definition update_message_proccessed (msg:Message) (v:Voter) := 
+  {|
+    id:=msg.(id)
+    ;block:=msg.(block)
+;kind := msg.(kind)
+;round:=msg.(round)
+    ;time:=msg.(time)
+    ;voter:=msg.(voter)
+    ;processed_by:= Dictionary.add Nat.eqb msg.(id) UnitC msg.(processed_by)
+  |}.
+
+
+
+Lemma message_to_vote_aux (msg:Message) 
+  {bizantiners_number last_block_number: nat} 
+  (voters: Voters bizantiners_number )
+  (last_block:Block last_block_number)
+  : option (Vote voters last_block).
+Proof.
+  destruct msg eqn:msg_eq.
+  pose (List.find (Nat.eqb voter0) (voters_to_list voters)) as find_eq.
+  destruct find_eq eqn:find_is.
+  2: refine None.
+  subst find_eq.
+  apply (find_some _ _ )in find_is.
+  destruct find_is as [in_proof is_voter].
+  rewrite Nat.eqb_eq in is_voter.
+  rewrite <- is_voter in in_proof.
+  destruct (is_prefix last_block (projT2 block0)) eqn:blocks_eq.
+  2: refine None.
+  apply is_prefix_implies_prefix in blocks_eq.
+  refine (Some(VoteC _ last_block voter0 in_proof _ blocks_eq)).
+Qed.
+  
+(* Expected to be used in messages with precommit votes*)
+Definition message_to_precommit_vote (msg:Message) 
+  {bizantiners_number last_block_number: nat} 
+  (voters: Voters bizantiners_number )
+  (last_block:Block last_block_number)
+  : option(Vote voters last_block ) := 
+  match msg.(kind) with
+  | PreCommitMessage => message_to_vote_aux msg voters last_block
+  | _ => None
+  end.
+
+Definition message_to_preview_vote (msg:Message) 
+  {bizantiners_number last_block_number: nat} 
+  (voters: Voters bizantiners_number )
+  (last_block:Block last_block_number)
+  : option(Vote voters last_block ) := 
+  match msg.(kind) with
+  | PreViewMessage => message_to_vote_aux msg voters last_block
+  | _ => None
+  end.
+
